theories/approxis/examples/pubkey.v
@@ -1,23 +1,13 @@
 From Ltac2 Require Import Ltac2.
 Set Default Proof Mode "Classic".
 From clutch.prob_lang Require Import advantage typing.tychk.
-From clutch.approxis Require Import approxis map list option.
+From clutch.approxis Require Import approxis map list option reltac2.
 From clutch.approxis.examples Require Import symmetric security_aux sum_seq xor prf advantage_laws.
 Set Default Proof Using "All".
 
-
 Section pubkey.
 
-(* Public key OTS-CPA$ security (one-time secrecy chosen plaintext attack -
-   real/random). *)
-
-(* Definition rand_cipher := λ:"msg",
-       let: "b" := rnd #() in
-       let: "x" := rnd #() in
-       let, ("B", "X") := (g^"b", g^"x") in
-       ("B", "X"). *)
-
-(* Context `{!approxisRGS Σ}. *)
+(* Public key real/random chosen plaintext attack and one-time security. *)
 
 Context (pkey : ∀ `{!approxisRGS Σ}, lrel Σ).
 Context (skey : ∀ `{!approxisRGS Σ}, lrel Σ).
@@ -41,7 +31,7 @@ Definition CPA_rand (Q : Z) : expr :=
 
 Definition CPA_real (Q : Z) : expr :=
   let, ("sk", "pk") := keygen #() in
-  let: "challenge" := enc "pk" in
+  let: "challenge" := λ:"msg", enc "pk" "msg" in
   let: "challenge" := q_calls_poly #() #() #Q "challenge" in
   ("pk", "challenge").
 
@@ -54,67 +44,55 @@ Definition hybrid (h Q : Z) : val :=
     let: "counter" := ref #0 in
     let: "challenge" :=
       λ: "msg",
-        if: (! "counter" < #Q) then
-          "counter" <- !"counter" + #1 ;;
-          if: (! "counter" < #h) then
+        let: "count" := ! "counter" in
+        if: ("count" < #Q) then
+          "counter" <- "count" + #1 ;;
+          if: ("count" < #h) then
             SOME (enc "pk" "msg")
-          else if: (! "counter" = #h) then
+          else if: ("count" = #h) then
                  "challenge" "msg"
                else SOME (rand_cipher "msg")
         else NONE
-
-        (* if: (! "counter" < #h)
-           then SOME (enc "pk" "msg")
-           else if: (! "counter" = #h) then
-                  ("challenge" "msg")
-                else if: (! "counter" < #Q)
-                     then SOME (rand_cipher "msg")
-                     else NONE *)
-
     in
     ("pk", "challenge").
 
 Definition τ_cpa `{!approxisRGS Σ} := (pkey _ _ * (msg _ _ → lrel_option (cipher _ _)))%lrel.
 
 Lemma hybrid_typed `{!approxisRGS Σ} h Q : ⊢ REL hybrid h Q << hybrid h Q : τ_cpa → τ_cpa.
-Proof with (rel_pures_r ; rel_pures_l).
-  rel_arrow_val.
-  rewrite /τ_cpa.
-  lrintro "pk challenge".
-  rewrite /hybrid...
-  rel_alloc_l counter_l as "counter_l" ; rel_alloc_r counter_r as "counter_r"...
-  iApply (refines_na_alloc ( ∃ (q : Z), counter_l ↦ #q ∗ counter_r ↦ₛ #q)%I
-            (nroot.@"pk")).
+Proof with ireds.
+  rel_arrow_val. rewrite /τ_cpa. lrintro "pk challenge". rewrite /hybrid...
+  iApply (refines_na_alloc ( ∃ (q : Z), counter ↦ #q ∗ counterₛ ↦ₛ #q)%I (nroot.@"pk")).
   iSplitL ; [iFrame|].
-  iIntros "#Hinv".
-  rel_vals => //.
-  iIntros (m_l m_r) "!> #m"...
+  iIntros "#Hinv". rel_vals => //. iIntros (m_l m_r) "!> #m"...
   iApply (refines_na_inv with "[$Hinv]"); [done|].
-  iIntros "(> (%q & counter_l & counter_r) & Hclose)".
-  rel_load_l ; rel_load_r...
-
-  destruct_decide (@bool_decide_reflect ((q < Q)%Z) _) as qQ...
-  - rel_load_l ; rel_load_r ; rel_store_l ; rel_store_r ; rel_load_l ; rel_load_r...
-    destruct_decide (@bool_decide_reflect (q+1 < h)%Z _) as qh...
+  iIntros "(> (%q & counter & counterₛ) & Hclose)"...
+  case_bool_decide as qQ...
+  2: iApply (refines_na_close with "[-]") ; iFrame ; rel_vals.
+  case_bool_decide as qh...
+  - iApply (refines_na_close with "[-]") ; iFrame.
+    rel_bind_l (enc _ _) ; rel_bind_r (enc _ _) ; iApply refines_bind => /=.
+    1: repeat rel_apply refines_app => //.
+    1: iApply enc_typed.
+    all: iIntros ; ireds ; rel_vals.
+  - case_bool_decide as qh'...
     + iApply (refines_na_close with "[-]") ; iFrame.
-      rel_bind_l (enc _ _) ; rel_bind_r (enc _ _) ; iApply refines_bind.
-      2:{ iIntros => /=... rel_vals. }
-      repeat rel_apply refines_app => //. 2,3: rel_vals.
-      iApply enc_typed.
-    + rel_load_l ; rel_load_r...
-      destruct_decide (@bool_decide_reflect (#(q+1) = #h)%Z _) as qh'...
-      * iApply (refines_na_close with "[-]") ; iFrame.
       rel_bind_l (challenge_l _) ; rel_bind_r (challenge_r _) ; iApply refines_bind.
       2:{ iIntros => /=... rel_vals. }
       by iApply "challenge".
-      * iApply (refines_na_close with "[-]") ; iFrame.
-        rel_bind_l (rand_cipher _) ; rel_bind_r (rand_cipher _) ; iApply refines_bind.
-        2:{ iIntros => /=... rel_vals. }
-        rel_apply refines_app.
-        1: iApply rand_cipher_typed.
-        rel_vals.
-  - iApply (refines_na_close with "[-]") ; iFrame.
-    rel_vals.
+    + iApply (refines_na_close with "[-]") ; iFrame.
+      rel_bind_l (rand_cipher _) ; rel_bind_r (rand_cipher _) ; iApply refines_bind.
+      2:{ iIntros => /=... rel_vals. }
+      rel_apply refines_app.
+      1: iApply rand_cipher_typed.
+      rel_vals.
+Qed.
+
+Lemma enc_eta_typed `{approxisRGS Σ} pk_l pk_r :
+  pkey _ _ pk_l pk_r
+    ⊢ REL (λ:"msg", enc pk_l "msg")%V << (λ:"msg", enc pk_r "msg")%V : msg _ _ → cipher _ _.
+Proof.
+  iIntros. rel_arrow_val. iIntros. rel_pures_l ; rel_pures_r.
+  repeat rel_apply refines_app. 1: iApply enc_typed. all: rel_vals.
 Qed.
 
 Lemma CPA_real_typed `{!approxisRGS Σ} Q : ⊢ REL CPA_real Q << CPA_real Q : τ_cpa.
@@ -123,11 +101,8 @@ Proof with (rel_pures_r ; rel_pures_l).
   rel_bind_l (keygen _) ; rel_bind_r (keygen _) ; iApply refines_bind => /=.
   1: rel_apply refines_app ; [iApply keygen_typed|rel_vals].
   lrintro "sk pk"...
-  rel_bind_l (enc _) ; rel_bind_r (enc _) ; iApply refines_bind => /=.
-  1: rel_apply refines_app ; [iApply enc_typed|rel_vals].
-  iIntros (m_l m_r) "#m"...
   rel_bind_l (q_calls_poly _ _ _ _) ; rel_bind_r (q_calls_poly _ _ _ _) ; rel_apply refines_bind.
-  1: iApply q_calls_poly_sem_typed_app ; rel_vals.
+  1: iApply q_calls_poly_sem_typed_app. 1: iApply enc_eta_typed. 1: done.
   iIntros (challenge_l challenge_r) "challenge"...
   rel_vals => //.
 Qed.
@@ -144,177 +119,147 @@ Proof with (rel_pures_r ; rel_pures_l).
   rel_vals => //.
 Qed.
 
-(* Base case for CPA_real. *)
-Fact cpa_hyb_real Q `{!approxisRGS Σ} :
-  ⊢ REL CPA_real Q << (hybrid Q Q CPA_OTS_real) : τ_cpa.
-Proof with (rel_pures_r ; rel_pures_l).
-  rewrite /CPA_OTS_real. rewrite /CPA_real.
+Fact hybrid_OTS_rand_typed k Q `{!approxisRGS Σ} :
+  ⊢ REL (hybrid k Q CPA_OTS_rand) << (hybrid k Q CPA_OTS_rand) : τ_cpa.
+Proof.
+  rel_apply refines_app. 1: iApply hybrid_typed. rewrite /CPA_OTS_rand. iApply CPA_rand_typed.
+Qed.
+
+Fact cpa_hyb_real_alt Q `{!approxisRGS Σ} :
+  ⊢ REL CPA_real Q << (hybrid Q Q CPA_OTS_rand) : τ_cpa.
+Proof with iredpures.
+  rewrite /CPA_OTS_rand. rewrite /CPA_real/CPA_rand.
   rel_bind_l (keygen _) ; rel_bind_r (keygen _) ; iApply refines_bind => /=.
   1: rel_apply refines_app ; [iApply keygen_typed|rel_vals].
   lrintro "sk pk"...
-  rel_bind_l (enc _) ; rel_bind_r (enc _) ; iApply refines_bind => /=.
-  1: rel_apply refines_app ; [iApply enc_typed|rel_vals].
-  iIntros (enc_pk_l enc_pk_r) "#enc_pk"...
-  rewrite {2}/q_calls_poly...
-  rel_alloc_r counter_ots as "counter_ots"...
-  rewrite /hybrid...
-  rel_alloc_r counter_hybrid as "counter_hybrid"...
+  rewrite {2}/q_calls_poly... rel_alloc_r counter_ots as "counter_ots"...
+  rewrite /hybrid... rel_alloc_r counter_hybrid as "counter_hybrid"...
   rewrite /q_calls_poly... rel_alloc_l counter_cpa as "counter_cpa"...
-
-  iApply (refines_na_alloc ( ∃ (q : Z), counter_cpa ↦ #q ∗ counter_hybrid ↦ₛ #q
-                                          ∗ (⌜q < Q⌝ -∗ counter_ots ↦ₛ #0)%Z
-            )%I
-            (nroot.@"pk")).
+  iApply (refines_na_alloc ( ∃ (q : Z), counter_cpa ↦ #q ∗ counter_hybrid ↦ₛ #q ∗ (⌜q < Q⌝ -∗ counter_ots ↦ₛ #0)%Z)%I (nroot.@"pk")).
   iSplitL ; [iFrame;easy|].
-  iIntros "#Hinv".
-  rel_vals => //.
-  iIntros (m_l m_r) "!> #m"...
+  iIntros "#Hinv". rel_vals => //. iIntros (m_l m_r) "!> #m"...
+  iApply (refines_na_inv with "[$Hinv]"); [done|].
+  iIntros "(> (%q & counter_cpa & counter_hybrid & counter_ots) & Hclose)" ; ireds.
+  case_bool_decide as qh...
+  2:{ iApply (refines_na_close with "[-]") ; iFrame. rel_vals. }
+  ireds. destruct_decide (@bool_decide_reflect (q < Q)%Z _)... 2: lia.
+  iApply (refines_na_close with "[-]").
+  iFrame "Hclose". iSplitL.
+  { iExists (q+1)%Z. iFrame. iIntros "!> ?". iApply "counter_ots". done. }
+  rel_bind_l (enc pk_l _) ; rel_bind_r (enc pk_r _) ; iApply refines_bind.
+  2: iIntros (c_l c_r) "#c" => /=... 2: rel_vals.
+  repeat rel_apply refines_app ; [iApply enc_typed | rel_vals..].
+Qed.
+
+Fact cpa_hyb_real_alt' Q `{!approxisRGS Σ} :
+  ⊢ REL (hybrid Q Q CPA_OTS_rand) << CPA_real Q : τ_cpa.
+Proof with iredpures.
+  rewrite /CPA_OTS_rand. rewrite /CPA_real/CPA_rand.
+  rel_bind_l (keygen _) ; rel_bind_r (keygen _) ; iApply refines_bind => /=.
+  1: rel_apply refines_app ; [iApply keygen_typed|rel_vals].
+  lrintro "sk pk"...
+  rewrite {1}/q_calls_poly... rel_alloc_l counter_ots as "counter_ots"...
+  rewrite /hybrid... rel_alloc_l counter_hybrid as "counter_hybrid"...
+  rewrite /q_calls_poly... rel_alloc_r counter_cpa as "counter_cpa"...
+  iApply (refines_na_alloc ( ∃ (q : Z), counter_cpa ↦ₛ #q ∗ counter_hybrid ↦ #q ∗ (⌜q < Q⌝ -∗ counter_ots ↦ #0)%Z)%I (nroot.@"pk")).
+  iSplitL ; [iFrame;easy|].
+  iIntros "#Hinv". rel_vals => //. iIntros (m_l m_r) "!> #m"...
   iApply (refines_na_inv with "[$Hinv]"); [done|].
   iIntros "(> (%q & counter_cpa & counter_hybrid & counter_ots) & Hclose)"...
-  rel_load_l ; rel_load_r...
-  set (h := Q).
-  destruct_decide (@bool_decide_reflect (q < h)%Z _) as qh...
-  2:{ iApply (refines_na_close with "[-]") ; iFrame.
-      rel_vals. }
-  rel_load_l ; rel_load_r ; rel_store_l ; rel_store_r ; rel_load_r...
-  destruct_decide (@bool_decide_reflect (q+1 < h)%Z _) as Sqh...
-  - iApply (refines_na_close with "[-]").
-    iFrame "Hclose". iSplitL.
-    { iExists (q+1)%Z. iFrame.
-      iIntros "!> h". iApply "counter_ots". iPureIntro. lia. }
-    rel_bind_l (enc_pk_l _) ; rel_bind_r (enc pk_r _) ; iApply refines_bind.
-    2: iIntros (c_l c_r) "#c" => /=... 2: rel_vals.
-    iSpecialize ("enc_pk" with "m").
-    (* TODO what to do with enc_pk here? *)
-    admit.
-  - rel_load_r... destruct_decide (@bool_decide_reflect (#(q+1) = #h)%Z _) as qh'...
-    2:{ subst h.
-        exfalso. assert (q+1 = Q -> False)%Z as SqQ. { intros <-. apply qh'. done. }
-        apply SqQ. lia. }
-    iSpecialize ("counter_ots" $! qh).
-    rel_load_r... rel_load_r ; rel_store_r...
-    iApply (refines_na_close with "[-]") ; iFrame...
-    iSplitL.
-    { iIntros "!> %". done. }
-    rel_bind_l (enc_pk_l _) ; rel_bind_r (enc_pk_r _) ; iApply refines_bind.
-    1: iApply "enc_pk" => //.
-    iIntros (c_l c_r) "#c" => /=...
-    rel_vals.
-Admitted.
+  ireds. case_bool_decide as qh...
+  2:{ iApply (refines_na_close with "[-]") ; iFrame. rel_vals. }
+  ireds. case_bool_decide... 2: lia.
+  iApply (refines_na_close with "[-]").
+  iFrame "Hclose". iSplitL.
+  { iExists (q+1)%Z. iFrame. iIntros "!> h". iApply "counter_ots". done. }
+  rel_bind_l (enc pk_l _) ; rel_bind_r (enc pk_r _) ; iApply refines_bind.
+  2: iIntros (c_l c_r) "#c" => /=... 2: rel_vals.
+  repeat rel_apply refines_app. 2,3: rel_vals. iApply enc_typed.
+Qed.
 
-(* just symmetry *)
-Fact cpa_hyb_real' Q `{!approxisRGS Σ} :
-  ⊢ REL (hybrid Q Q CPA_OTS_real) << CPA_real Q : τ_cpa.
-Admitted.
-
-Fact cpa_hyb_rand Q `{!approxisRGS Σ} :
+(* Base case for CPA_rand. *)
+Fact cpa_hyb_rand_alt Q `{!approxisRGS Σ} :
   ⊢ REL CPA_rand Q << (hybrid 0 Q CPA_OTS_rand) : τ_cpa.
-Proof with (rel_pures_r ; rel_pures_l).
-  rewrite /CPA_OTS_rand. rewrite /CPA_rand.
+Proof with iredpures.
+  rewrite /CPA_OTS_rand. rewrite /CPA_real/CPA_rand.
   rel_bind_l (keygen _) ; rel_bind_r (keygen _) ; iApply refines_bind => /=.
   1: rel_apply refines_app ; [iApply keygen_typed|rel_vals].
   lrintro "sk pk"...
-  rewrite {2}/q_calls_poly...
-  rel_alloc_r counter_ots as "counter_ots"...
-  rewrite /hybrid...
-  rel_alloc_r counter_hybrid as "counter_hybrid"...
+  rewrite {2}/q_calls_poly... rel_alloc_r counter_ots as "counter_ots"...
+  rewrite /hybrid... rel_alloc_r counter_hybrid as "counter_hybrid"...
   rewrite /q_calls_poly... rel_alloc_l counter_cpa as "counter_cpa"...
-
-  iApply (refines_na_alloc ( ∃ (q : Z), ⌜0 <= q⌝%Z ∗ counter_cpa ↦ #q ∗ counter_hybrid ↦ₛ #q
-                                          ∗ (⌜q = 0⌝ -∗ counter_ots ↦ₛ #0)%Z)%I
-            (nroot.@"pk")).
+  iApply (refines_na_alloc ( ∃ (q : Z), counter_cpa ↦ #q ∗ counter_hybrid ↦ₛ #q ∗ (⌜q = 0⌝ -∗ counter_ots ↦ₛ #0)%Z
+                                        ∗ ⌜0 <= q⌝%Z)%I (nroot.@"pk")).
   iSplitL ; [iFrame;easy|].
-  iIntros "#Hinv".
-  rel_vals => //.
-  iIntros (m_l m_r) "!> #m"...
+  iIntros "#Hinv". rel_vals => //. iIntros (m_l m_r) "!> #m"...
   iApply (refines_na_inv with "[$Hinv]"); [done|].
-  iIntros "(> (%q & %qpos & counter_cpa & counter_hybrid & counter_ots) & Hclose)"...
-  rel_load_l ; rel_load_r...
-  set (h := 0%Z).
-  destruct_decide (@bool_decide_reflect (q < Q)%Z _) as qh...
-  2:{ iApply (refines_na_close with "[-]") ; iFrame. iSplitR. 1: done.
-      rel_vals. }
-  rel_load_l ; rel_load_r ; rel_store_l ; rel_store_r ; rel_load_r...
-  destruct_decide (@bool_decide_reflect (q+1 < h)%Z _) as Sqh...
-  - iApply (refines_na_close with "[-]").
+  iIntros "(> (%q & counter_cpa & counter_hybrid & counter_ots & %qpos) & Hclose)"...
+  ireds. case_bool_decide as qh...
+  2:{ iApply (refines_na_close with "[-]") ; iFrame. iSplitR ; [done|]. rel_vals. }
+  ireds. case_bool_decide... 1: lia.
+  case_bool_decide as eq_q_0...
+  2:{
+    iApply (refines_na_close with "[-]").
     iFrame "Hclose". iSplitL.
-    { iExists (q+1)%Z. iFrame. iSplitR. 1: iPureIntro ; lia.
-      iIntros "!> %hh". lia. }
-    exfalso. lia.
-  - rel_load_r... destruct_decide (@bool_decide_reflect (#(q+1) = #h)%Z _) as qh'...
-    2:{ subst h.
-        iApply (refines_na_close with "[-]") ; iFrame "Hclose"...
-        iSplitL.
-        { iIntros "!>". iExists (q+1)%Z. iFrame. iSplitR. 1: iPureIntro ; lia.
-          iIntros "%hh". lia. }
-        rel_bind_l (rand_cipher _) ; rel_bind_r (rand_cipher _) ; iApply refines_bind.
-        2:{ iIntros => /=... rel_vals. }
-        rel_apply refines_app.
-        1: iApply rand_cipher_typed.
-        rel_vals.
-    }
-    subst h.
-    inversion qh'. lia.
+    { iExists (q+1)%Z. iFrame. iSplitL. 2: iPureIntro ; lia. iIntros "!> %h". lia. }
+    rel_bind_l (rand_cipher _) ; rel_bind_r (rand_cipher _) ; iApply refines_bind.
+    2:{ iIntros => /=... rel_vals. }
+    rel_apply refines_app. 1: iApply rand_cipher_typed. rel_vals.
+  }
+  inversion eq_q_0 as [q0].
+  iSpecialize ("counter_ots" $! eq_refl). ireds.
+  iApply (refines_na_close with "[-]"). iFrame "Hclose". iSplitL.
+  { iExists (q+1)%Z. subst. iFrame. iSplitL. 2: iPureIntro ; lia. iIntros "!> %h". lia. }
+  rel_bind_l (rand_cipher _) ; rel_bind_r (rand_cipher _) ; iApply refines_bind.
+  2:{ iIntros => /=... rel_vals. }
+  rel_apply refines_app. 1: iApply rand_cipher_typed. rel_vals.
 Qed.
 
-Fact cpa_hyb_rand' Q `{!approxisRGS Σ} :
+Fact cpa_hyb_rand_alt' Q `{!approxisRGS Σ} :
   ⊢ REL (hybrid 0 Q CPA_OTS_rand) << CPA_rand Q : τ_cpa.
-Proof with (rel_pures_r ; rel_pures_l).
-  rewrite /CPA_OTS_rand. rewrite /CPA_rand.
+Proof with iredpures.
+  rewrite /CPA_OTS_rand. rewrite /CPA_real/CPA_rand.
   rel_bind_l (keygen _) ; rel_bind_r (keygen _) ; iApply refines_bind => /=.
   1: rel_apply refines_app ; [iApply keygen_typed|rel_vals].
   lrintro "sk pk"...
-  rewrite {1}/q_calls_poly...
-  rel_alloc_l counter_ots as "counter_ots"...
-  rewrite /hybrid...
-  rel_alloc_l counter_hybrid as "counter_hybrid"...
+  rewrite {1}/q_calls_poly... rel_alloc_l counter_ots as "counter_ots"...
+  rewrite /hybrid... rel_alloc_l counter_hybrid as "counter_hybrid"...
   rewrite /q_calls_poly... rel_alloc_r counter_cpa as "counter_cpa"...
-
-  iApply (refines_na_alloc ( ∃ (q : Z), ⌜0 <= q⌝%Z ∗ counter_cpa ↦ₛ #q ∗ counter_hybrid ↦ #q
-                                          ∗ (⌜q = 0⌝ -∗ counter_ots ↦ #0)%Z)%I
-            (nroot.@"pk")).
+  iApply (refines_na_alloc ( ∃ (q : Z), counter_cpa ↦ₛ #q ∗ counter_hybrid ↦ #q ∗ (⌜q = 0⌝ -∗ counter_ots ↦ #0)%Z
+                                        ∗ ⌜0 <= q⌝%Z)%I (nroot.@"pk")).
   iSplitL ; [iFrame;easy|].
-  iIntros "#Hinv".
-  rel_vals => //.
-  iIntros (m_l m_r) "!> #m"...
+  iIntros "#Hinv". rel_vals => //. iIntros (m_l m_r) "!> #m"...
   iApply (refines_na_inv with "[$Hinv]"); [done|].
-  iIntros "(> (%q & %qpos & counter_cpa & counter_hybrid & counter_ots) & Hclose)"...
-  rel_load_l ; rel_load_r...
-  set (h := 0%Z).
-  destruct_decide (@bool_decide_reflect (q < Q)%Z _) as qh...
-  2:{ iApply (refines_na_close with "[-]") ; iFrame. iSplitR. 1: done.
-      rel_vals. }
-  rel_load_l ; rel_load_r ; rel_store_l ; rel_store_r ; rel_load_l...
-  destruct_decide (@bool_decide_reflect (q+1 < h)%Z _) as Sqh...
-  - iApply (refines_na_close with "[-]").
-    iFrame "Hclose". iSplitL.
-    { iExists (q+1)%Z. iFrame. iSplitR. 1: iPureIntro ; lia.
-      iIntros "!> %hh". lia. }
-    exfalso. lia.
-  - rel_load_l... destruct_decide (@bool_decide_reflect (#(q+1) = #h)%Z _) as qh'...
-    2:{ subst h.
-        iApply (refines_na_close with "[-]") ; iFrame "Hclose"...
-        iSplitL.
-        { iIntros "!>". iExists (q+1)%Z. iFrame. iSplitR. 1: iPureIntro ; lia.
-          iIntros "%hh". lia. }
-        rel_bind_l (rand_cipher _) ; rel_bind_r (rand_cipher _) ; iApply refines_bind.
-        2:{ iIntros => /=... rel_vals. }
-        rel_apply refines_app.
-        1: iApply rand_cipher_typed.
-        rel_vals.
-    }
-    subst h.
-    inversion qh'. lia.
+  iIntros "(> (%q & counter_cpa & counter_hybrid & counter_ots & %qpos) & Hclose)"...
+  ireds. case_bool_decide as qh...
+  2:{ iApply (refines_na_close with "[-]") ; iFrame. iSplitR ; [done|]. rel_vals. }
+  ireds. case_bool_decide... 1: lia.
+  case_bool_decide as eq_q_0...
+  2:{
+    iApply (refines_na_close with "[-]"). iFrame "Hclose". iSplitL.
+    { iExists (q+1)%Z. iFrame. iSplitL. 2: iPureIntro ; lia. iIntros "!> %h". lia. }
+    rel_bind_l (rand_cipher _) ; rel_bind_r (rand_cipher _) ; iApply refines_bind.
+    2:{ iIntros => /=... rel_vals. }
+    rel_apply refines_app. 1: iApply rand_cipher_typed. rel_vals.
+  }
+  inversion eq_q_0 as [q0].
+  iSpecialize ("counter_ots" $! eq_refl). ireds.
+  iApply (refines_na_close with "[-]"). iFrame "Hclose". iSplitL.
+  { iExists (q+1)%Z. subst. iFrame. iSplitL. 2: iPureIntro ; lia. iIntros "!> %h". lia. }
+  rel_bind_l (rand_cipher _) ; rel_bind_r (rand_cipher _) ; iApply refines_bind.
+  2:{ iIntros => /=... rel_vals. }
+  rel_apply refines_app. 1: iApply rand_cipher_typed. rel_vals.
 Qed.
+
 
 Context (adversary : val).
 Context (adversary_typed : forall `{!approxisRGS Σ}, ⊢ REL adversary << adversary : τ_cpa → lrel_bool).
 
 Definition ε_OTS h Q b := advantage (λ:"v", adversary (hybrid h Q "v")) CPA_OTS_real CPA_OTS_rand #b.
 
-Fact foo h Q (b : bool) :
+Fact advantage_hybrid_OTS h Q (b : bool) :
   (advantage adversary (hybrid h Q CPA_OTS_real) (hybrid h Q CPA_OTS_rand) #b <= ε_OTS h Q b)%R.
-Proof with (rel_pures_r ; rel_pures_l).
+Proof.
   apply advantage_reduction_lr. intros.
   exists τ_cpa, τ_cpa.
   intuition auto.
@@ -324,110 +269,176 @@ Proof with (rel_pures_r ; rel_pures_l).
 Qed.
 
 (* Switch back from rand to real by stepping k. *)
-(* TODO prove one of these *)
-Fact cpa_hyb_real_rand Q k `{!approxisRGS Σ} :
-  ⊢ REL (hybrid k Q CPA_OTS_rand) << (hybrid (k+1) Q CPA_OTS_real) : τ_cpa.
-Proof with (rel_pures_r ; rel_pures_l).
-  rewrite /CPA_OTS_real/CPA_real...
-  rewrite /CPA_OTS_rand/CPA_rand...
+Fact cpa_hyb_real_rand Q k (kpos : (0 <= k)%Z) `{!approxisRGS Σ} :
+  ⊢ REL (hybrid k Q CPA_OTS_real) << (hybrid (k+1) Q CPA_OTS_rand) : τ_cpa.
+Proof with iredpures.
+  rewrite /CPA_OTS_real/CPA_real... rewrite /CPA_OTS_rand/CPA_rand...
   rel_bind_l (keygen _) ; rel_bind_r (keygen _) ; iApply refines_bind => /=.
   1: rel_apply refines_app ; [iApply keygen_typed|rel_vals].
   lrintro "sk pk"...
-  rewrite {1}/q_calls_poly...
-  rel_alloc_l counter_ots_l as "counter_ots_l"...
-  rewrite {1}/hybrid...
-  rel_alloc_l counter_hyb_l as "counter_hyb_l"...
-  (* how to progress with enc pk_r on the right? *)
-Admitted.
+  rewrite {1}/q_calls_poly... rel_alloc_l counter_ots_l as "counter_ots_l"...
+  rewrite {1}/hybrid... rel_alloc_l counter_hyb_l as "counter_hyb_l"...
+  rewrite {1}/q_calls_poly... rel_alloc_r counter_ots_r as "counter_ots_r"...
+  rewrite {1}/hybrid... rel_alloc_r counter_hyb_r as "counter_hyb_r"...
+  iApply (refines_na_alloc ( ∃ (q q_ots_l q_ots_r : Z),
+                (counter_hyb_l ↦ #q ∗ counter_hyb_r ↦ₛ #q
+                ∗ counter_ots_l ↦ #q_ots_l ∗ counter_ots_r ↦ₛ #q_ots_r)
+                ∗ (⌜ 0 <= q ∧
+                     (q <= k -> (q_ots_l = 0 ∧ q_ots_r = 0)) ∧
+                     (q = k+1 -> q_ots_r < 1)%Z⌝ )%Z)%I
+            (nroot.@"pk")).
+  iSplitL ; [iFrame|]. 1: iPureIntro ; intuition auto ; try lia.
+  iIntros "#Hinv". rel_vals => //. iIntros (m_l m_r) "!> #m"...
+  iApply (refines_na_inv with "[$Hinv]"); [done|].
+  iIntros "(> (%q & %q_ots_l & %q_ots_r & (counter_cpa & counter_hybrid & counter_ots_l & counter_ots_r) & %rest) & Hclose)".
+  ireds. case_bool_decide as lt_q_Q...
+  2:{ iApply (refines_na_close with "[-]") ; iFrame. iSplitR. 1: done. rel_vals. }
+  ireds. case_bool_decide as lt_q_k...
+  - case_bool_decide as lt_q_Sk... 2: lia.
+    iApply (refines_na_close with "[-]") ; iFrame.
+    iSplitL ; [iFrame|]. 1: iPureIntro ; intuition auto ; try lia.
+    rel_bind_l (enc pk_l _) ; rel_bind_r (enc pk_r _) ; iApply refines_bind.
+    2: iIntros (c_l c_r) "#c" => /=... 2: rel_vals.
+    repeat rel_apply refines_app. 2,3: rel_vals. iApply enc_typed.
+  - case_bool_decide as eq_q_k...
+    + inversion eq_q_k. ireds.
+      destruct rest as (q_pos & xyz).
+      assert (q_ots_l = 0). { apply xyz. lia. }
+      case_bool_decide... 2: lia.
+      case_bool_decide... 2: lia.
+      ireds. iApply (refines_na_close with "[-]") ; iFrame.
+      iSplitL ; [iFrame|]. 1: iPureIntro ; intuition auto ; try lia.
+      rel_bind_l (enc pk_l _) ; rel_bind_r (enc pk_r _) ; iApply refines_bind.
+      2: iIntros (c_l c_r) "#c" => /=... 2: rel_vals.
+      repeat rel_apply refines_app. 2,3: rel_vals. iApply enc_typed.
+    + assert (q ≠ k). 1: intros -> ; by apply eq_q_k.
+      case_bool_decide as lt_q_Sk... 1: lia.
+      case_bool_decide as eq_q_Sk...
+      * ireds. destruct rest as (q_pos & ql & qr).
+        inversion eq_q_Sk as [eq_q_Sk'].
+        case_bool_decide as lt_q_qts_r... 2: lia.
+        ireds. iApply (refines_na_close with "[-]") ; iFrame.
+        iSplitL ; [iFrame|]. 1: iPureIntro ; intuition auto ; try lia.
+        rel_bind_l (rand_cipher _) ; rel_bind_r (rand_cipher _) ; iApply refines_bind.
+        2:{ iIntros => /=... rel_vals. }
+        rel_apply refines_app. 1: iApply rand_cipher_typed. rel_vals.
+      * iApply (refines_na_close with "[-]") ; iFrame.
+        iSplitL ; [iFrame|]. 1: iPureIntro ; intuition auto ; try lia.
+        rel_bind_l (rand_cipher _) ; rel_bind_r (rand_cipher _) ; iApply refines_bind.
+        2:{ iIntros => /=... rel_vals. }
+        rel_apply refines_app. 1: iApply rand_cipher_typed. rel_vals.
+Qed.
 
 (* Symmetric to above. *)
-Fact cpa_hyb_real_rand' Q k `{!approxisRGS Σ} :
-  ⊢ REL (hybrid (k+1) Q CPA_OTS_real) << (hybrid k Q CPA_OTS_rand) : τ_cpa.
-Admitted.
-
-(* TODO prove one of these *)
-Lemma induction_base_lr Q `{!approxisRGS Σ} :
-  ⊢ REL (hybrid 0 Q CPA_OTS_real) << (hybrid 0 Q CPA_OTS_rand) : τ_cpa.
+Fact cpa_hyb_real_rand' Q k (kpos : (0 <= k)%Z) `{!approxisRGS Σ} :
+  ⊢ REL (hybrid (k+1) Q CPA_OTS_rand) << (hybrid k Q CPA_OTS_real) : τ_cpa.
 Proof with (rel_pures_r ; rel_pures_l).
-  rewrite /CPA_OTS_real/CPA_real...
-  rewrite /CPA_OTS_rand/CPA_rand...
+  rewrite /CPA_OTS_real/CPA_real... rewrite /CPA_OTS_rand/CPA_rand...
   rel_bind_l (keygen _) ; rel_bind_r (keygen _) ; iApply refines_bind => /=.
   1: rel_apply refines_app ; [iApply keygen_typed|rel_vals].
   lrintro "sk pk"...
-  (* Same problem with enc pk_l as above. *)
-Admitted.
+  rewrite {1}/q_calls_poly... rel_alloc_l counter_ots_l as "counter_ots_l"...
+  rewrite {1}/hybrid... rel_alloc_l counter_hyb_l as "counter_hyb_l"...
+  rewrite {1}/q_calls_poly... rel_alloc_r counter_ots_r as "counter_ots_r"...
+  rewrite {1}/hybrid... rel_alloc_r counter_hyb_r as "counter_hyb_r"...
+  iApply (refines_na_alloc ( ∃ (q q_ots_l q_ots_r : Z),
+                (counter_hyb_l ↦ #q ∗ counter_hyb_r ↦ₛ #q
+                ∗ counter_ots_l ↦ #q_ots_l ∗ counter_ots_r ↦ₛ #q_ots_r)
+                ∗ (⌜ 0 <= q ∧
+                     (q <= k -> (q_ots_l = 0 ∧ q_ots_r = 0)) ∧
+                     (q = k+1 -> q_ots_l < 1)%Z⌝ )%Z)%I
+            (nroot.@"pk")).
+  iSplitL ; [iFrame|]. 1: iPureIntro ; intuition auto ; try lia.
+  iIntros "#Hinv". rel_vals => //. iIntros (m_l m_r) "!> #m"...
+  iApply (refines_na_inv with "[$Hinv]"); [done|].
+  iIntros "(> (%q & %q_ots_l & %q_ots_r & (counter_cpa & counter_hybrid & counter_ots_l & counter_ots_r) & %rest) & Hclose)".
+  ireds. case_bool_decide as lt_q_Q...
+  2:{ iApply (refines_na_close with "[-]") ; iFrame. iSplitR. 1: done. rel_vals. }
+  ireds. destruct_decide (@bool_decide_reflect ((q < k)%Z) _) as lt_q_k...
+  - case_bool_decide as lt_q_Sk... 2: lia.
+    iApply (refines_na_close with "[-]") ; iFrame.
+    iSplitL ; [iFrame|]. 1: iPureIntro ; intuition auto ; try lia.
+    rel_bind_l (enc pk_l _) ; rel_bind_r (enc pk_r _) ; iApply refines_bind.
+    2: iIntros (c_l c_r) "#c" => /=... 2: rel_vals.
+    repeat rel_apply refines_app. 2,3: rel_vals. iApply enc_typed.
+  - destruct_decide (@bool_decide_reflect (#q = #k) _) as eq_q_k...
+    + inversion eq_q_k.
+      ireds. destruct rest as (q_pos & xyz).
+      assert (q_ots_l = 0). { apply xyz. lia. }
+      case_bool_decide... 2: lia.
+      case_bool_decide... 2: lia.
+      ireds. iApply (refines_na_close with "[-]") ; iFrame.
+      iSplitL ; [iFrame|]. 1: iPureIntro ; intuition auto ; try lia.
+      rel_bind_l (enc pk_l _) ; rel_bind_r (enc pk_r _) ; iApply refines_bind.
+      2: iIntros (c_l c_r) "#c" => /=... 2: rel_vals.
+      repeat rel_apply refines_app. 2,3: rel_vals. iApply enc_typed.
+    + assert (q ≠ k). 1: intros -> ; by apply eq_q_k.
+      case_bool_decide as lt_q_Sk... 1: lia.
+      case_bool_decide as eq_q_Sk...
+      * ireds. destruct rest as (q_pos & ql & qr).
+        inversion eq_q_Sk as [eq_q_Sk'].
+        case_bool_decide as lt_q_qts_r... 2: lia.
+        rel_load_l ; rel_store_l...
+        iApply (refines_na_close with "[-]") ; iFrame.
+        iSplitL ; [iFrame|]... 1: iPureIntro ; intuition auto ; try lia.
+        rel_bind_l (rand_cipher _) ; rel_bind_r (rand_cipher _) ; iApply refines_bind.
+        2:{ iIntros => /=... rel_vals. }
+        rel_apply refines_app. 1: iApply rand_cipher_typed. rel_vals.
+      * iApply (refines_na_close with "[-]") ; iFrame.
+        iSplitL ; [iFrame|]... 1: iPureIntro ; intuition auto ; try lia.
+        rel_bind_l (rand_cipher _) ; rel_bind_r (rand_cipher _) ; iApply refines_bind.
+        2:{ iIntros => /=... rel_vals. }
+        rel_apply refines_app. 1: iApply rand_cipher_typed. rel_vals.
+Qed.
 
-(* symmetric *)
-Lemma induction_base_lr' Q `{!approxisRGS Σ} :
-  ⊢ REL (hybrid 0 Q CPA_OTS_rand) << (hybrid 0 Q CPA_OTS_real) : τ_cpa.
-Admitted.
-
-Lemma induction_base Q (b : bool) :
-  (nonneg (advantage adversary (hybrid 0 Q CPA_OTS_real) (hybrid 0 Q CPA_OTS_rand) #b) <= 0)%R.
-Proof. eapply (lr_advantage _ _ _ _ adversary_typed (@induction_base_lr Q) (@induction_base_lr' Q)). Qed.
 
 (* TODO define ε' instead of assuming it exists. *)
 (* the fact that ε_OTS varies with Q is annoying in the proof; we can just take ε' to be the max over ε_OTS. *)
 Variable ε' : forall (Q : Z) (b : bool), R.
 Hypothesis (ε_max : forall Q (b : bool) k, (ε_OTS k Q b <= ε' Q b)%R).
 
-
-Lemma Claim_15_5_aux (Q : Z) (k : nat) (b : bool) :
-  (advantage adversary (hybrid k Q CPA_OTS_real) (hybrid 0 Q CPA_OTS_rand) #b
-   <= k * ε' Q b)%R.
+Lemma Claim_15_5_aux_alt (Q : Z) (k : nat) (b : bool) :
+  (advantage adversary (hybrid 0 Q CPA_OTS_rand) (hybrid k Q CPA_OTS_rand) #b <= k * ε' Q b)%R.
 Proof.
   intros. set (ε := ε' Q b). induction k.
-  - replace (0%nat * ε)%R with 0%R by real_solver. 1: eapply induction_base.
+  - replace (0%nat * ε)%R with 0%R. 2: real_solver. replace (_ 0%nat) with 0%Z by lia.
+    eapply lr_advantage_reflexive.
+    1: apply adversary_typed. apply hybrid_OTS_rand_typed.
   - replace (S k) with (k + 1) by lia.
     replace (INR (k+1)) with (INR k + 1)%R by real_solver.
-    eapply (advantage_triangle _ _ _ _ _ ε (k*ε)). 3: lra.
-    2: apply IHk. clear IHk.
-    opose proof (lr_advantage _ _ _ _ adversary_typed (@cpa_hyb_real_rand' _ _) (@cpa_hyb_real_rand _ _) b)
-      as step.
-    replace ε with (0+ε)%R by lra.
-    eapply advantage_triangle. 3: reflexivity.
-    2:{ etrans. 2: apply ε_max.
-        opose proof (foo k Q b) as bar. rewrite advantage_sym in bar. apply bar. }
+    eapply (advantage_triangle _ _ _ _ _ (k*ε) ε). 3: lra.
+    1: apply IHk. clear IHk.
+    replace ε with (ε+0)%R by lra.
+    eapply (advantage_triangle _ _ (hybrid k Q CPA_OTS_real) _ _ ε 0%R) => //.
+    { etrans. 2: apply ε_max.
+      opose proof (advantage_hybrid_OTS k Q b) as bar. rewrite advantage_sym. apply bar. }
     replace (Z.of_nat (k+1)) with (k + 1)%Z by lia.
+    opose proof (lr_advantage _ _ _ _ adversary_typed (@cpa_hyb_real_rand Q k _) (@cpa_hyb_real_rand' _ _ _) b)
+      as step.
+    1,2: lia.
     apply step.
 Qed.
 
+Lemma cpa_hyb_real_adv_alt (b : bool) Q :
+  (nonneg (advantage adversary (CPA_real Q) (hybrid Q Q CPA_OTS_rand) #b) <= 0)%R.
+Proof. apply (lr_advantage _ _ _ _ adversary_typed (@cpa_hyb_real_alt Q) (@cpa_hyb_real_alt' Q)). Qed.
 
-Lemma cpa_hyb_real_adv (b : bool) Q :
-  (nonneg (advantage adversary (CPA_real Q) (hybrid Q Q CPA_OTS_real) #b) <= 0)%R.
-Proof. eapply (lr_advantage _ _ _ _ adversary_typed (@cpa_hyb_real Q) (@cpa_hyb_real' Q)). Qed.
-
-Lemma cpa_hyb_rand_adv (b : bool) Q :
-  (nonneg (advantage adversary (hybrid 0 Q CPA_OTS_rand) (CPA_rand Q) #b) <= 0)%R.
-Proof. eapply (lr_advantage _ _ _ _ adversary_typed (@cpa_hyb_rand' Q) (@cpa_hyb_rand Q)). Qed.
+Lemma cpa_hyb_rand_adv_alt (b : bool) Q :
+  (nonneg (advantage adversary (CPA_rand Q) (hybrid 0 Q CPA_OTS_rand) #b) <= 0)%R.
+Proof. apply (lr_advantage _ _ _ _ adversary_typed (@cpa_hyb_rand_alt Q) (@cpa_hyb_rand_alt' Q)). Qed.
 
 Lemma Claim_15_5 (Q : nat) (b : bool) :
     (advantage adversary (CPA_real Q) (CPA_rand Q) #b <= Q * ε' Q b)%R.
 Proof.
   intros.
   eapply advantage_triangle.
-  1: apply cpa_hyb_real_adv.
+  1: apply cpa_hyb_real_adv_alt.
   1: eapply advantage_triangle.
-  2: apply cpa_hyb_rand_adv.
-  1: apply Claim_15_5_aux.
-  1: reflexivity. field_simplify. done.
+  2: rewrite advantage_sym.
+  2: apply cpa_hyb_rand_adv_alt.
+  1: rewrite advantage_sym.
+  1: apply Claim_15_5_aux_alt.
+  1: reflexivity. field_simplify. reflexivity.
 Qed.
-
-
-(* A CPA_real ~ A (hybrid Q Q CPA_OTS.real)
-
-   A (hybrid h Q CPA_OTS.real) ~ A (hybrid h Q CPA_OTS.rand)
-   because
-   A (hybrid h Q CPA_OTS.real)
-   =   (A ∘ hybrid h Q) CPA_OTS.real
-   ~ε~ (A ∘ hybrid h Q) CPA_OTS.rand
-   =   A (hybrid h Q CPA_OTS.rand)
-
-   where ε = adv (A ∘ hybrid h Q) CPA_OTS.real CPA_OTS.rand
-   although this should also hold for
-   ε' = adv A CPA_OTS.real CPA_OTS.rand
-   since (A ∘ hybrid h Q) can't distinguish the games except at the h-th query.
-   In other words, it should be possible to prove ε = ε'.
-   But even ε is an advantage against a single-time security game, so maybe that's good enough. *)
 
 End pubkey.
